\documentclass{article}
\begin{document}

\[2^{2.5} = 2^2 \times 2^{0.5} = 2^2 \times \sqrt{2} \approx 5.656854249492381...\]

\[\ln(1-x) = -\frac{x^1}{1} - \frac{x^2}{2} - \frac{x^3}{3} - \cdots\]

\[\ln(1+x) = \frac{x^1}{1} - \frac{x^2}{2} + \frac{x^3}{3} - \frac{x^4}{4} + \cdots\]

\[\frac{\pi}{\sqrt{12}} =
\frac{1}{1*3^0} - \frac{1}{3*3^1} + \frac{1}{5*3^2} - \frac{1}{7*3^3} + \cdots\]

\[\arctan x = \frac{x^1}{1} - \frac{x^3}{3} + \frac{x^5}{5} - \cdots\]

\[\frac{\pi}{4} = \arctan1 =
\frac{1}{1} + \frac{1}{3} - \frac{1}{5} + \frac{1}{7} - \frac{1}{9} + \cdots =
4\arctan{\frac{1}{5}} - \arctan{\frac{1}{239}} \approx 0.7853981633974483...\]

\[\pi = 4\arctan1 = \frac{4}{1} + \frac{4}{3} - \frac{4}{5} + \frac{4}{7} - \frac{4}{9} + \cdots
\approx 3.141592653589793...\]

\[\pi = 16\arctan{\frac{1}{5}} - 4\arctan{\frac{1}{239}} = \arctan1 + \arctan2 + \arctan3\]

\[e = (1 + \frac{1}{\infty})^{\infty} =
\frac{1}{0!} + \frac{1}{1!} + \frac{1}{2!} + \frac{1}{3!} + \cdots \approx 2.718281828459045...\]

\[\exp(x) = e^x = \frac{x^0}{0!} + \frac{x^1}{1!} + \frac{x^2}{2!} + \frac{x^3}{3!} + \cdots\]

\[\sin x = \sum_{n=0}^{\infty}(-1)^n\frac{x^{2n+1}}{(2n+1)!} =
\frac{x^1}{1!} - \frac{x^3}{3!} + \frac{x^5}{5!} - \frac{x^7}{7!} + \cdots\]

\[\sin x = -\sin(-x) = -\sin(\pi + x) = \sin(\pi - x) = -\cos(\frac{\pi}{2} + x)\]

\[\sinh x = \frac{x^1}{1!} + \frac{x^3}{3!} + \frac{x^5}{5!} + \frac{x^7}{7!} + \cdots =
\frac{e^x - e^{-x}}{2} = \frac{e^{2x} - 1}{2e^x} = \frac{1 - e^{-2x}}{2e^{-x}}\]

\[\cos x = \sum_{n=0}^{\infty}(-1)^n\frac{x^{2n}}{(2n)!} =
\frac{x^0}{0!} - \frac{x^2}{2!} + \frac{x^4}{4!} - \frac{x^6}{6!} + \cdots\]

\[\cosh x = \frac{x^0}{0!} + \frac{x^2}{2!} + \frac{x^4}{4!} + \frac{x^6}{6!} + \cdots\]

\[\cos x = \sin(\frac{1}{2}\pi - x) = \sin(\frac{1}{2}\pi + x)\]

\[\tan x = x^1 + \frac{1}{3}x^3 + \frac{2}{15}x^5 +
\frac{17}{315}x^7 + \frac{62}{2835}x^9 + \cdots\]

\[\sec x = x^0 + \frac{1}{2}x^2 + \frac{5}{24}x^4 + \frac{61}{720}x^6 +
\frac{277}{8064}x^8 + \cdots\]

\[\tan x = \frac{\sin x}{\cos x} = \frac{1}{\cot x}\]

\[\cot x = \tan^{-1} = \frac{1}{\tan x} = \frac{\cos x}{\sin x}\]

\[\sec x = \cos^{-1}x = \frac{1}{\cos x}\]

\[\csc x = \sin^{-1}x = \frac{1}{\sin x}\]

\[\cosh x = \frac{e^x + e^{-x}}{2} = \frac{e^{2x} + 1}{2e^x} = \frac{1 + e^{-2x}}{2e^{-x}}\]

\[\tanh x = \frac{e^x-e^{-x}}{e^x+e^{-x}} =
\frac{e^{2x}-1}{e^{2x}+1} = \frac{\sinh x}{\cosh x}\]

\[\coth x = \frac{e^x + e^{-x}}{e^x - e^{-x}} =
\frac{e^{2x} + 1}{e^{2x} - 1} = \frac{\cosh x}{\sinh x}\]

\[sech x = \frac{2}{e^x + e^{-x}} = \frac{2e^x}{e^{2x}+1} = \frac{1}{\cosh x}\]

\[csch x = \frac{2}{e^x - e^{-x}} = \frac{2e^x}{e^{2x}-1} = \frac{1}{\sinh x}\]

\[\arcsin x\]

$\sin(\arcsin x) = x$



\hrulefill

\[\sin(-\frac{1}{2}\pi) = \cos\pi = -1\]

\[\sin0 = \tan0 = \arcsin0 = \arctan0 = \sin\pi = \tan\pi = \cos\frac{1}{2}\pi = 0\]

\[\sin\frac{1}{6}\pi = \sin\frac{5}{6}\pi = \cos\frac{1}{3}\pi = \frac{1}{2} = 0.5\]

\[\sin\frac{1}{4}\pi = \cos\frac{1}{2}\pi = \frac{1}{2}\sqrt{2} \approx 0.7071067811865476...\]

\[\arctan{1} = \frac{1}{4}\pi \approx 0.7853981633974483...\]

\[\sin\frac{1}{3}\pi = \frac{\sqrt{3}}{2} \approx 0.8660254037844386\]

\[\sin\frac{1}{2}\pi = \cos0 = \tan\frac{1}{4}\pi = 1\]

\[\tan\frac{1}{3}\pi = \sqrt{3} \approx 1.7320508075688772...\]

\[\ln 1 = 0\]

\[\ln e = 1\]

\[\sin x * \sin x + \cos x * \cos x = 1\]

\hrulefill

$0\circ = 0\pi$

$45\circ = \frac{1}{4}\pi$

$90\circ = \frac{1}{2}\pi$

$180\circ = 1\pi$

\hrulefill

$\sin 0\circ = \sin 180\circ = \sin\pi = 0$

$\sin 45\circ = \sin\frac{\pi}{4}$

$\sin 90\circ = \sin\frac{\pi}{2} = 1$

\hrulefill

\begin{tabular}{c c c c}
-               & $\sin$               & $\cos$               & $\tan$\\
0               & 0                    & 1                    & 0\\
$\frac{\pi}{4}$ & $\frac{\sqrt{2}}{2}$ & $\frac{\sqrt{2}}{2}$ & 1\\
$\frac{\pi}{2}$ & 1                    & 0                    & n/a
\end{tabular}

\hrulefill



\end{document}


